lakefile.lean
@@ -3,8 +3,9 @@ open Lake DSL
 
 package lean_tla
 
-require mathlib from git "https://github.com/leanprover-community/mathlib4.git"
 require cslib from git "https://github.com/leanprover/cslib" @ "main"
+
+require mathlib from git "https://github.com/leanprover-community/mathlib4.git"
 
 @[default_target]
 lean_lib TlaDsl
